got type translation working, proved it preserves well-formed types

src/Cps_Trans.v
@@ -1,16 +1,58 @@
-Require Import Core_Definitions Source_Definitions.
+Require Import Core_Infrastructure Source_Definitions Target_Definitions
+               Source_Properties Target_Properties.
 
 Definition dummy_type := t_typ_bool.
 
-Fixpoint cps_type_trans (s:typ) : typ :=
-match s with
-| s_typ_bool => t_typ_bool
-| s_typ_arrow s1 s2 =>
-  t_typ_arrow (t_typ_pair (cps_type_trans s1)
-                          (t_typ_arrow (cps_type_trans s2) (t_typ_bvar 1)))
-              (t_typ_bvar 0)
-| _ => dummy_type
-end.
+Lemma s_type_arrow_inv_l : forall s1 s2,
+ s_type (s_typ_arrow s1 s2) -> s_type s1.
+Proof. inversion 1. assumption. Qed.
+
+Lemma s_type_arrow_inv_r : forall s1 s2,
+ s_type (s_typ_arrow s1 s2) -> s_type s2.
+Proof. inversion 1. assumption. Qed.
+
+Definition cps_type_trans (s:typ) (wf : s_type s) : typ.
+ induction s; try solve [elimtype False; inversion wf].
+ (* bool+ = bool *)
+ exact t_typ_bool.
+ (* (s1->s2)+ = forall a, s1+ X ((s2+ -> a) -> a) *)
+ exact (t_typ_arrow (t_typ_pair (IHs1 (s_type_arrow_inv_l s1 s2 wf))
+                                (t_typ_arrow (IHs2 (s_type_arrow_inv_r s1 s2 wf))
+                                             (t_typ_bvar 1)))
+                    (t_typ_bvar 0)).
+Defined.
+
+Lemma cps_type_trans_bool : forall wf,
+  cps_type_trans s_typ_bool wf = t_typ_bool.
+Proof. auto. Qed.
+
+Lemma cps_type_trans_arrow : forall s1 s2 wf,
+  cps_type_trans (s_typ_arrow s1 s2) wf = 
+  t_typ_arrow (t_typ_pair (cps_type_trans s1 (s_type_arrow_inv_l s1 s2 wf))
+                          (t_typ_arrow
+                            (cps_type_trans s2 (s_type_arrow_inv_r s1 s2 wf))
+                            (t_typ_bvar 1)))
+              (t_typ_bvar 0).
+Proof. intros. simpl. f_equal. Qed.
+
+Lemma cps_type_trans_produces_t_type : forall s wf_s,
+  t_type (cps_type_trans s wf_s).
+Proof.
+  induction s; intros; auto; try solve [elimtype False; inversion wf_s].
+  rewrite cps_type_trans_arrow.
+  apply_fresh t_type_arrow as X. simpl.
+  apply t_type_pair.
+  rewrite open_tt_rec_t_type; apply IHs1.
+  apply_fresh t_type_arrow as Y.
+  rewrite open_tt_rec_t_type; rewrite open_tt_rec_t_type; apply IHs2.
+  apply t_type_var. apply t_type_var.
+Qed.
+
+Extraction cps_type_trans. (* BAM *)
+
+Definition cps_type_trans_computation (s : typ) (wf : s_type s) :=
+  t_typ_arrow (t_typ_arrow (cps_type_trans s wf) (t_typ_bvar 1))
+              (t_typ_bvar 0).
 
 Eval simpl in cps_type_trans (s_typ_arrow s_typ_bool s_typ_bool).
 
